$$
\left[\begin{matrix}ξ_{0}\end{matrix}\right]
$$

$$
\lVert\xi\rVert=ξ_{0}
$$

$$
M(\xi)=\left[\begin{matrix}ξ_{0}\end{matrix}\right]
$$

$$
\left[\begin{matrix}ξ_{0} & ξ_{1}\\- ξ_{1} & ξ_{0}\end{matrix}\right]
$$

$$
\lVert\xi\rVert=\sqrt{ξ_{0}^{2}+ξ_{1}^{2}}
$$

$$
M(\xi)^2=\left[\begin{matrix}ξ_{0}^{2} - ξ_{1}^{2} & 2 ξ_{0} ξ_{1}\\- 2 ξ_{0} ξ_{1} & ξ_{0}^{2} - ξ_{1}^{2}\end{matrix}\right]
$$

$$
\left[\begin{matrix}ξ_{0} & ξ_{1} & ξ_{2}\\- ξ_{2} & ξ_{0} & ξ_{1}\\- ξ_{1} & - ξ_{2} & ξ_{0}\end{matrix}\right]
$$

$$
\lVert\xi\rVert=\sqrt[3]{ξ_{0}^{3} + 3 ξ_{0} ξ_{1} ξ_{2} - ξ_{1}^{3} + ξ_{2}^{3}}
$$

$$
M(\xi)^3=\left[\begin{matrix}ξ_{0}^{3} - 6 ξ_{0} ξ_{1} ξ_{2} - ξ_{1}^{3} + ξ_{2}^{3} & 3 ξ_{0}^{2} ξ_{1} - 3 ξ_{0} ξ_{2}^{2} - 3 ξ_{1}^{2} ξ_{2} & 3 ξ_{0}^{2} ξ_{2} + 3 ξ_{0} ξ_{1}^{2} - 3 ξ_{1} ξ_{2}^{2}\\- 3 ξ_{0}^{2} ξ_{2} - 3 ξ_{0} ξ_{1}^{2} + 3 ξ_{1} ξ_{2}^{2} & ξ_{0}^{3} - 6 ξ_{0} ξ_{1} ξ_{2} - ξ_{1}^{3} + ξ_{2}^{3} & 3 ξ_{0}^{2} ξ_{1} - 3 ξ_{0} ξ_{2}^{2} - 3 ξ_{1}^{2} ξ_{2}\\- 3 ξ_{0}^{2} ξ_{1} + 3 ξ_{0} ξ_{2}^{2} + 3 ξ_{1}^{2} ξ_{2} & - 3 ξ_{0}^{2} ξ_{2} - 3 ξ_{0} ξ_{1}^{2} + 3 ξ_{1} ξ_{2}^{2} & ξ_{0}^{3} - 6 ξ_{0} ξ_{1} ξ_{2} - ξ_{1}^{3} + ξ_{2}^{3}\end{matrix}\right]
$$

$$
\left[\begin{matrix}ξ_{0} & ξ_{1} & ξ_{2} & ξ_{3}\\- ξ_{3} & ξ_{0} & ξ_{1} & ξ_{2}\\- ξ_{2} & - ξ_{3} & ξ_{0} & ξ_{1}\\- ξ_{1} & - ξ_{2} & - ξ_{3} & ξ_{0}\end{matrix}\right]
$$

$$
\lVert\xi\rVert=\sqrt[4]{ξ_{0}^{4} + 4 ξ_{0}^{2} ξ_{1} ξ_{3} + 2 ξ_{0}^{2} ξ_{2}^{2} - 4 ξ_{0} ξ_{1}^{2} ξ_{2} + 4 ξ_{0} ξ_{2} ξ_{3}^{2} + ξ_{1}^{4} + 2 ξ_{1}^{2} ξ_{3}^{2} - 4 ξ_{1} ξ_{2}^{2} ξ_{3} + ξ_{2}^{4} + ξ_{3}^{4}}
$$

$$
\left[\begin{matrix}ξ_{0} & ξ_{1} & ξ_{2} & ξ_{3} & ξ_{4}\\- ξ_{4} & ξ_{0} & ξ_{1} & ξ_{2} & ξ_{3}\\- ξ_{3} & - ξ_{4} & ξ_{0} & ξ_{1} & ξ_{2}\\- ξ_{2} & - ξ_{3} & - ξ_{4} & ξ_{0} & ξ_{1}\\- ξ_{1} & - ξ_{2} & - ξ_{3} & - ξ_{4} & ξ_{0}\end{matrix}\right]
$$

$$
\left[\begin{matrix}ξ_{0} & ξ_{1} & ξ_{2} & ξ_{3} & ξ_{4} & ξ_{5}\\- ξ_{5} & ξ_{0} & ξ_{1} & ξ_{2} & ξ_{3} & ξ_{4}\\- ξ_{4} & - ξ_{5} & ξ_{0} & ξ_{1} & ξ_{2} & ξ_{3}\\- ξ_{3} & - ξ_{4} & - ξ_{5} & ξ_{0} & ξ_{1} & ξ_{2}\\- ξ_{2} & - ξ_{3} & - ξ_{4} & - ξ_{5} & ξ_{0} & ξ_{1}\\- ξ_{1} & - ξ_{2} & - ξ_{3} & - ξ_{4} & - ξ_{5} & ξ_{0}\end{matrix}\right]
$$

$$
\left[\begin{matrix}ξ_{0} & ξ_{1} & ξ_{2} & ξ_{3} & ξ_{4} & ξ_{5} & ξ_{6}\\- ξ_{6} & ξ_{0} & ξ_{1} & ξ_{2} & ξ_{3} & ξ_{4} & ξ_{5}\\- ξ_{5} & - ξ_{6} & ξ_{0} & ξ_{1} & ξ_{2} & ξ_{3} & ξ_{4}\\- ξ_{4} & - ξ_{5} & - ξ_{6} & ξ_{0} & ξ_{1} & ξ_{2} & ξ_{3}\\- ξ_{3} & - ξ_{4} & - ξ_{5} & - ξ_{6} & ξ_{0} & ξ_{1} & ξ_{2}\\- ξ_{2} & - ξ_{3} & - ξ_{4} & - ξ_{5} & - ξ_{6} & ξ_{0} & ξ_{1}\\- ξ_{1} & - ξ_{2} & - ξ_{3} & - ξ_{4} & - ξ_{5} & - ξ_{6} & ξ_{0}\end{matrix}\right]
$$

$$
\begin{pmatrix}-\lambda & 1 & 0 & 0 & 0 & 0 & 0 & 0\\1 & -\lambda & 0 & 1 & 0 & 0 & 0 & 0\\0 & 0 & -\lambda & 0 & 0 & 1 & 0 & 0\\0 & 0 & 0 & -\lambda & 0 & 0 & 0 & 1\\0 & 0 & 1 & 0 & -\lambda & 0 & 0 & 0\\0 & 0 & 0 & 0 & 0 & -\lambda & 0 & 0\\0 & 0 & 0 & 0 & 0 & 0 & -\lambda & 0\\0 & 0 & 0 & 0 & 1 & 0 & 0 & -\lambda\\\end{pmatrix}
$$

$$
\begin{pmatrix}-\lambda & 1 & 0 & 0 & 0 & 0 & 0 & 0 & 0 & 0 & 0 & 0 & 0 & 0\\1 & -\lambda & 0 & 1 & 0 & 0 & 0 & 0 & 0 & 0 & 0 & 0 & 0 & 0\\0 & 0 & -\lambda & 0 & 0 & 1 & 0 & 0 & 0 & 0 & 0 & 0 & 0 & 0\\0 & 0 & 0 & -\lambda & 0 & 0 & 0 & 1 & 0 & 0 & 0 & 0 & 0 & 0\\0 & 0 & 1 & 0 & -\lambda & 0 & 0 & 0 & 0 & 1 & 0 & 0 & 0 & 0\\0 & 0 & 0 & 0 & 0 & -\lambda & 0 & 0 & 0 & 0 & 0 & 1 & 0 & 0\\0 & 0 & 0 & 0 & 0 & 0 & -\lambda & 0 & 0 & 0 & 0 & 0 & 0 & 1\\0 & 0 & 0 & 0 & 1 & 0 & 0 & -\lambda & 0 & 0 & 0 & 0 & 0 & 0\\0 & 0 & 0 & 0 & 0 & 0 & 0 & 0 & -\lambda & 0 & 0 & 0 & 0 & 0\\0 & 0 & 0 & 0 & 0 & 0 & 0 & 0 & 0 & -\lambda & 0 & 0 & 0 & 0\\0 & 0 & 0 & 0 & 0 & 0 & 1 & 0 & 0 & 0 & -\lambda & 0 & 0 & 0\\0 & 0 & 0 & 0 & 0 & 0 & 0 & 0 & 0 & 0 & 0 & -\lambda & 0 & 0\\0 & 0 & 0 & 0 & 0 & 0 & 0 & 0 & 0 & 0 & 0 & 0 & -\lambda & 0\\0 & 0 & 0 & 0 & 0 & 0 & 0 & 0 & 1 & 0 & 0 & 0 & 0 & -\lambda\\\end{pmatrix}
$$
